Reduce the number of jump tables in closure stubs
By moving one to a top level function instead of in 2 * max_app
different places.

The proofs build, but are cheated. The new definitions most likely have
a bug or two still.

compiler/backend/clos_to_bvlScript.sml
@@ -140,14 +140,25 @@ val build_recc_lets_def = Define `
 
 val num_stubs_def = Define `
   num_stubs max_app =
-    (* generic apps *)         max_app
+    (* partial app labels *)   1
+    (* generic apps *)       + max_app
     (* partial apps *)       + max_app * max_app
     (* equality of values *) + 1n
     (* equality of blocks *) + 1
-    (* ToList *)             + 1`;
+    (* ToList *)             + 1
+    (* Empty, because the must be an odd number *) + 1`;
+
+val get_partial_app_label_fn_location_def = Define `
+  get_partial_app_label_fn_location = 0n`;
+
+val generic_app_fn_location_def = Define `
+  generic_app_fn_location n = n + 1n`;
+
+val partial_app_fn_location_def = Define `
+  partial_app_fn_location (max_app:num) m n = 1 + max_app + max_app * m + n`;
 
 val equality_location_def = Define`
-  equality_location (max_app:num) = max_app + max_app * max_app`;
+  equality_location (max_app:num) = 1 + max_app + max_app * max_app`;
 
 val block_equality_location_def = Define`
   block_equality_location max_app = equality_location max_app + 1`;
@@ -159,10 +170,22 @@ val mk_cl_call_def = Define `
   mk_cl_call cl args =
     If (Op Equal [mk_const (LENGTH args - 1); mk_el cl (mk_const 1)])
        (Call (LENGTH args - 1) NONE (args ++ [cl] ++ [mk_el cl (mk_const 0)]))
-       (Call 0 (SOME (LENGTH args - 1)) (args ++ [cl]))`;
+       (Call 0 (SOME (generic_app_fn_location (LENGTH args - 1))) (args ++ [cl]))`;
 
-val partial_app_fn_location_def = Define `
-  partial_app_fn_location (max_app:num) m n = max_app + max_app * m + n`;
+val get_partial_app_label_fn_def = Define `
+  get_partial_app_label_fn max_app =
+    (* Call this stub function with two arguments, the total number of arguments
+     * the closure wants, and the ones already there. Both must be 1 less than
+     * the actual value, since there is no possibility of 0 total or partial
+     * arguments *)
+    Jump (Var 0)
+      (GENLIST
+        (\total_args.
+          (Jump (Var 2)
+            (GENLIST
+              (\prev_args. mk_label (partial_app_fn_location max_app total_args prev_args))
+              max_app)))
+        max_app)`;
 
 (* Generic application of a function to n+1 arguments *)
 val generate_generic_app_def = Define `
@@ -173,9 +196,10 @@ val generate_generic_app_def = Define `
             (Jump (mk_el (Var (n+2)) (mk_const 1))
               (GENLIST (\num_args.
                  Let [Call num_args
-                           NONE (GENLIST (\arg. Var (arg + 2 + n - num_args)) (num_args + 1) ++
-                                 [Var (n + 3)] ++
-                                 [mk_el (Var (n + 3)) (mk_const 0)])]
+                           NONE
+                           (GENLIST (\arg. Var (arg + 2 + n - num_args)) (num_args + 1) ++
+                            [Var (n + 3)] ++
+                            [mk_el (Var (n + 3)) (mk_const 0)])]
                    (mk_cl_call (Var 0) (GENLIST (\n. Var (n + 3)) (n - num_args))))
                max_app))
             (* Partial application *)
@@ -184,10 +208,8 @@ val generate_generic_app_def = Define `
                 (* Partial application of a normal closure *)
                 (Op (Cons partial_app_tag)
                     (REVERSE
-                      (Jump (mk_el (Var (n+2)) (mk_const 1))
-                        (GENLIST (\total_args.
-                          mk_label (partial_app_fn_location max_app total_args n))
-                         max_app) ::
+                      (Call 0 (SOME get_partial_app_label_fn_location)
+                        [mk_const n; mk_el (Var (n+2)) (mk_const 1)] ::
                        Var 0 ::
                        Var (n + 2) ::
                        GENLIST (\n. Var (n + 1)) (n + 1))))
@@ -196,10 +218,8 @@ val generate_generic_app_def = Define `
                   (GENLIST (\prev_args.
                     Op (Cons partial_app_tag)
                        (REVERSE
-                         (Jump (Op Add [mk_const (n + prev_args + 2); Var 1])
-                            (GENLIST (\total_args.
-                              mk_label (partial_app_fn_location max_app total_args (n + prev_args + 1)))
-                             max_app) ::
+                         (Call 0 (SOME get_partial_app_label_fn_location)
+                            [mk_const (n + prev_args + 1); Op Add [mk_const (n + prev_args + 2); Var 1]] ::
                           Var 1 ::
                           mk_el (Var (n+3)) (mk_const 2) ::
                           GENLIST (\this_arg. Var (this_arg + 2)) (n+1) ++
@@ -251,7 +271,10 @@ val block_equality_code_def = Define`
 val init_code_def = Define `
   init_code max_app =
     sptree$fromList
-      (GENLIST (\n. (n + 2, generate_generic_app max_app n)) max_app ++
+      ((2, get_partial_app_label_fn max_app) ::
+       GENLIST (\n. (n + 2, generate_generic_app max_app n)) max_app ++
+               (* TODO: Shouldn't need the full complement. The number of
+                * partial args must be less than the total *)
                FLAT (GENLIST (\m. GENLIST (\n. (m - n + 1,
                                      generate_partial_app_closure_fn m n)) max_app) max_app) ++
        [equality_code max_app;
